Weidenbach_Book/Watched_Literals/Watched_Literals_Transition_System.thy
@@ -1,6 +1,6 @@
 theory Watched_Literals_Transition_System
   imports WB_More_Refinement CDCL.CDCL_W_Abstract_State
-    CDCL.CDCL_W_Restart  "../CDCL/Pragmatic_CDCL"
+    CDCL.CDCL_W_Restart  CDCL.Pragmatic_CDCL
 begin
 
 chapter \<open>Two-Watched Literals\<close>
